Turn on warn-redundant-assumptions

Source/DafnyStandardLibraries/examples/FunctionsExamples.dfy
@@ -2,25 +2,27 @@ module FunctionExamples {
 
   import opened DafnyStdLibs.Function
 
-  lemma TestInjective() {
-    assert Injective<int, int>((x) => x + 2);
-    var square := (x: int) => x * x;
+  const square := (x: int) => x * x
+  lemma TestInjective()
+    ensures Injective<int, int>((x) => x + 2)
+    ensures !Injective<int, int>((x) => x * x)
+  {
     assert square(-1) == square(1);
-    assert !Injective<int, int>((x) => x * x);
   }
 
-  lemma TestCommutative() {
-    assert Commutative<int, int>((x, y) => x + y);
-    var subtract := (x: int, y: int) => x - y;
+  const subtract := (x: int, y: int) => x - y
+  lemma TestCommutative()
+    ensures Commutative<int, int>((x, y) => x + y)
+    ensures !Commutative<int, int>(subtract)
+  {
     assert subtract(1,2) != subtract(2,1);
-    assert !Commutative<int, int>(subtract);
   }
 
-  lemma TestAssociative() {
-    assert Associative<int>((x, y) => x + y);
-    var subtract := (x: int, y: int) => x - y;
+  lemma TestAssociative()
+    ensures Associative<int>((x, y) => x + y)
+    ensures !Associative<int>(subtract)
+  {
     assert subtract(1,2) != subtract(2,1);
-    assert !Associative<int>(subtract);
   }
 
 }
