Source/DafnyStandardLibraries/examples/RelationExamples.dfy
@@ -2,42 +2,38 @@ module RelationExamples {
 
   import opened DafnyStdLibs.Relations
 
-  lemma TestRelationProperties() {
-    assert Reflexive<int>((a,b) => a == b);
-    assert Irreflexive<int>((a,b) => a != b);
-    assert Symmetric((a,b) => a && b);
-    assert Asymmetric<int>((a,b) => a < b);
-    assert AntiSymmetric<bool>((a,b) => a ==> b);
-    assert Connected<int>((a,b) => a < b);
-    assert StronglyConnected<int>((a,b) => a <= b);
-    assert Transitive<int>((a,b) => a == b);
-    assert TotalOrdering<int>((a,b) => a <= b);
-    assert StrictTotalOrdering<int>((a,b) => a < b);
-
-    var partialOrdering := (a: int, b: int) => !(a == 9 && b == 10) && a <= b;
-    assert PartialOrdering<int>(partialOrdering);
-    assert !partialOrdering(9,10) && !partialOrdering(10,9);
-    assert !StronglyConnected(partialOrdering);
-
-    assert TotalOrdering<int>((a,b) => a <= b);
-    assert StrictTotalOrdering<int>((a,b) => a < b);
-
-    assert EquivalenceRelation((a,b) => a % 2 == b % 2);
+  const partialOrdering := (a: int, b: int) => !(a == 9 && b == 10) && a <= b
+  lemma TestRelationProperties()
+    ensures Reflexive<int>((a,b) => a == b)
+    ensures Irreflexive<int>((a,b) => a != b)
+    ensures Symmetric((a,b) => a && b)
+    ensures Asymmetric<int>((a,b) => a < b)
+    ensures AntiSymmetric<bool>((a,b) => a ==> b)
+    ensures Connected<int>((a,b) => a < b)
+    ensures StronglyConnected<int>((a,b) => a <= b)
+    ensures Transitive<int>((a,b) => a == b)
+    ensures TotalOrdering<int>((a,b) => a <= b)
+    ensures StrictTotalOrdering<int>((a,b) => a < b)
+    ensures !StronglyConnected(partialOrdering)
+    ensures TotalOrdering<int>((a,b) => a <= b)
+    ensures StrictTotalOrdering<int>((a,b) => a < b)
+    ensures EquivalenceRelation((a,b) => a % 2 == b % 2)
+  {
+    assert !partialOrdering(9,10);
   }
 
-  lemma TestElementProperties() {
-    var xs := { 1, 2 };
-    var lessEqual := (a,b) => a <= b;
-    assert IsLeast(lessEqual, 1, xs);
-    assert IsMinimal(lessEqual, 1, xs);
+  const lessEqualInt := (a: int, b) => a <= b
+  lemma TestElementProperties()
+    ensures IsLeast(lessEqualInt, 1, { 1, 2 })
+    ensures IsMinimal(lessEqualInt, 1, { 1, 2 })
+  {
   }
 
-  lemma TestSorting() {
-    var xs := [1,2,3];
+  lemma TestSorting()
+    ensures SortedBy(lessEqualInt, [1, 2, 3])
+    ensures !SortedBy(lessEqualInt, [3, 2, 1])
+  {
     var ys := [3,2,1];
-    var lessEqual := (a,b) => a <= b;
-    assert SortedBy(lessEqual, xs);
     assert ys[0] > ys[1];
-    assert !SortedBy(lessEqual, ys);
   }
 }
